Gasm.lean
@@ -146,6 +146,7 @@ import Gasm.Compiler.Word.StructuredStraightLineAArch64.Differential
 import Gasm.Compiler.Word.StructuredStraightLineMicrosoftX64Entry
 import Gasm.Compiler.Word.StructuredConditionMicrosoftX64Entry
 import Gasm.Compiler.Word.StructuredConditionMicrosoftX64EntryControls
+import Gasm.Compiler.Word.StructuredConditionMicrosoftX64CFG
 import Gasm.Compiler.Word.StructuredStraightLineMicrosoftX64Entry.Differential
 import Gasm.Compiler.Word.Examples
 import Gasm.Compiler.TypedCFG
